---
layout: post
title: 常用傅里叶变换对及证明
date: 2019-10-31 11:20:00
Author: Lee-Coderr
categories: 
- 数学
tags: [FFT,数学]
comments: true
toc: true
pinned: true
---



# $\delta(t) \leftrightarrow 1$

## Proof：


$$
\begin{align*}
F(\omega)&=\int_{-\infty}^{+\infty} f(t) e^{-j \omega t} d t \\
&= \int_{0-}^{0+} \delta(t) e^{-j \omega t} d t \\
&= \int_{0-}^{0+} \delta(t) d t \\
&= 1
\end{align*}
$$


# $e^{-at}\varepsilon(t) \leftrightarrow \frac{1}{a+j\omega}$ (a>0)

## Proof：

$$
\begin{align*}
F(\omega)&=\int_{-\infty}^{+\infty} f(t) e^{-j \omega t} d t \\
&= \int_{0}^{+\infty} e^{-at} e^{-j \omega t} d t \\
&= \int_{0}^{+\infty} e^{-(a+j \omega) t} d t \\
&= \frac{1}{a+j\omega}
\end{align*}
$$

# $e^{-a|t|}\leftrightarrow \frac{2a}{a^2+\omega^2}$ (a>0)

## Proof：

$$
\begin{align*}
F(\omega)&=\int_{-\infty}^{+\infty} f(t) e^{-j \omega t} d t \\
&= \int_{-\infty}^{0} e^{at} e^{-j \omega t} d t + \int_{0}^{+\infty}e^{-at} e^{-j \omega t} d t \\
&= \frac{1}{a-j\omega} + \frac{1}{a+j\omega} \\
&= \frac{2a}{a^2+\omega^2}
\end{align*}
$$

# $1 \leftrightarrow 2\pi\delta(t)$

## Proof 1：

首先有：
$$
\lim_{a\rightarrow 0}  e^{-a\left | t \right |} = 1
$$

$$
\begin{align*}
F(\omega)&=\int_{-\infty}^{+\infty} f(t) e^{-j \omega t} d t \\
&= \int_{-\infty}^{+\infty} 1 \cdot e^{-j \omega t} d t \\
&= \int_{-\infty}^{+\infty} \lim_{a\rightarrow 0}  e^{-a\left | t \right |} \cdot e^{-j \omega t} d t \\
&= \lim_{a\rightarrow 0} \int_{-\infty}^{+\infty} e^{-a\left | t \right |} \cdot e^{-j \omega t} d t \\
&= \lim_{a\rightarrow 0} \frac{2a}{a^2+\omega^2} \\
&= 
\left\{\begin{matrix}
+\infty & \omega=0 \\ 
0 & \omega \neq 0
\end{matrix}\right. \\
&= k \delta(\omega)
\end{align*}
$$
$k $ 是未知数，现在要求 $k$ 。

由于 ：
$$
\begin{align*}
\lim_{a\rightarrow 0} \frac{2a}{a^2+\omega^2} 
&= k \delta(\omega)
\end{align*}
$$
两边求积分：
$$
\begin{align*}
k &= \lim_{a\rightarrow 0} \int_{-\infty}^{+\infty}\frac{2a}{a^2+\omega^2} d\omega \\
&= \lim_{a\rightarrow 0} \int_{-\infty}^{+\infty}\frac{2}{1+(\frac{\omega}{a})^2} d\frac{\omega}{a} \\
&= 2\lim_{a\rightarrow 0} [\arctan \frac{\omega}{a}]_{-\infty}^{+\infty} \\
&= 2 \pi
\end{align*}
$$
所以 ：
$$
1 \leftrightarrow 2\pi\delta(t)
$$

## Proof 2：

由 
$$
\delta(t) \leftrightarrow 1
$$
傅里叶反变换
$$
\begin{align*}
\delta(t) &= \frac{1}{2\pi}\int_{-\infty}^{+\infty}1 \cdot e^{j\omega t} d \omega\\
\end{align*}
$$
$\delta(t)$ 为偶函数：
$$
\begin{align*}
\delta(t) &= \delta(-t) \\
&= \frac{1}{2\pi}\int_{-\infty}^{+\infty}1 \cdot e^{-j\omega t} d \omega\\
\end{align*}
$$
所以 ：
$$
\begin{align*}
\int_{-\infty}^{+\infty}1 \cdot e^{-j\omega t} d \omega = 2\pi\delta(t) \\
\end{align*}
$$


# $\varepsilon(t) \leftrightarrow \pi \delta(\omega)+\frac{1}{j\omega}$

## Proof：

因为 ：
$$
\lim_{a\rightarrow 0}  e^{-at} = \varepsilon(t)
$$

$$
\begin{align*}
F(\omega)&=\int_{-\infty}^{+\infty} f(t) e^{-j \omega t} d t \\
&= \int_{-\infty}^{+\infty} \varepsilon(t) \cdot e^{-j \omega t} d t \\
&= \int_{-\infty}^{+\infty} \lim_{a\rightarrow 0}  e^{-at} \cdot e^{-j \omega t} d t \\
&= \lim_{a\rightarrow 0} \int_{-\infty}^{+\infty} e^{-at} \cdot e^{-j \omega t} d t \\
&= \lim_{a\rightarrow 0} \frac{1}{a+j\omega} \\
&= \lim_{a\rightarrow 0} (\frac{a}{a^2+\omega^2} - j\frac{\omega}{a^2+\omega^2}) \\
&= 
\left\{\begin{matrix}
+\infty & \omega=0 \\ 
0 & \omega \neq 0
\end{matrix}\right. + \frac{1}{j\omega}\\
&= k\delta(\omega) + \frac{1}{j\omega} \quad (k是未知数) \\
&= \pi \delta(\omega) + \frac{1}{j\omega} \quad (用积分求k值，见上方1\leftrightarrow 2\pi \delta 的Proof1)\\
\end{align*}
$$

